Name the type and fields of the result of a monadic computation on a bitstream (#97)
This should make models and proofs easier to read. Concretely, this PR
does the following:
* Introduce a type `datatype Result<A> = Result(value: A, rest:
Rand.Bitstream)`
* Change the definition of `Hurd` from `type Hurd<A> = Rand.Bitstream ->
(A, Rand.Bitstream)` to `type Hurd<A> = Rand.Bitstream -> Result<A>`

By submitting this pull request, I confirm that my contribution is made
under the terms of the [MIT
license](https://github.com/dafny-lang/dafny/blob/master/LICENSE.txt).

src/Distributions/Coin/Model.dfy
@@ -7,7 +7,7 @@ module Coin.Model {
   import Rand
   import Monad
 
-  function Sample(s: Rand.Bitstream): (bool, Rand.Bitstream) {
+  function Sample(s: Rand.Bitstream): Monad.Result<bool> {
     Monad.Coin(s)
   }
 }
